Playbook/hm.lean
@@ -1,131 +1,328 @@
 import Parser
-import Playbook.ffidecl
-
+import Playbook.dependentPP
 open Parser Parser.Char
+
+infixr : 60 " <$ " => Functor.mapConst
+infixr : 60 " $> " => flip Functor.mapConst
+
+abbrev Symbol := String
+
+inductive Expr where
+  | CI (i : Int)       | CS (s : String)        | CB (b : Bool) | CUnit
+  | App (e₁ e₂ : Expr) | Cond (e₁ e₂ e₃ : Expr) | Let (a : Symbol) (e₁ e₂ : Expr)
+  | Fix (e : Expr)     | Fixcomb (e : Expr)
+  | Var (s : Symbol)   | Fun (a : Symbol) (e : Expr)
+  | Prod' (e₁ e₂ : Expr)
+deriving Repr, BEq, Nonempty
+instance : Inhabited Expr := ⟨Expr.CUnit⟩
+
+abbrev Binding := Symbol × Expr
+
+inductive Associativity | leftAssoc | rightAssoc deriving Ord, Repr
+
+instance : ToString Associativity where
+  toString
+  | .leftAssoc => "left"
+  | .rightAssoc => "right"
+
+abbrev OpIndex := Nat × String
+instance opIndexOrd : Ord OpIndex where
+  compare 
+  | (n, a), (n', a') => 
+    let n := compare n' n; let a := compare a a'
+    if a matches .eq then .eq else n.then a
+
+/--(ℕ × String) ↦ ε × Associativity-/
+abbrev OpTable α := Std.TreeMap OpIndex ((α -> α -> α) × Associativity) opIndexOrd.compare
+
 namespace Lexing
-abbrev TParser := SimpleParser Substring Char
+
+open Std in
+
+abbrev TParser := SimpleParserT Substring Char $ StateM $ OpTable Expr
 
 abbrev INT := @ASCII.parseInt
 
 def alphanum' [Parser.Stream σ Char] [Parser.Error ε σ Char] [Monad m]
   : ParserT ε σ Char m Char :=
   withErrorMessage "expected letter or digit character or \'" do
-    tokenFilter fun c =>
-      if c >= 'a' then c <= 'z'
-      else if c >= 'A' then c <= 'Z'
-      else c >= '0' && c <= '9' || c == '\''
+    tokenFilter fun c => c.isAlphanum || c == '\'' || c == '_'
+def alpha' [Parser.Stream σ Char] [Parser.Error ε σ Char] [Monad m]
+  : ParserT ε σ Char m Char :=
+  withErrorMessage "expected alphabetic character" do
+    tokenFilter fun c => if c >= 'a' then c <= 'z' else c == '_' || c >= 'A' && c <= 'Z'
 
-def reserved := ["let", "in", "fn", "fun", "=", "if", "else", "then", "->"]
+def void : TParser α -> TParser Unit := (() <$ ·)
+
+def MLCOMMENTL := void $ string "(*"
+def MLCOMMENTR := void $ string "*)"
+
+def comment : TParser Unit :=
+  withBacktracking $
+   (string "NB.") *> dropUntil (endOfInput <|> void eol) anyToken
+
+def spaces : TParser Unit :=
+  dropMany <| MLCOMMENTR <|> MLCOMMENTL <|> void ASCII.whitespace <|> comment <|> void eol
+
+abbrev ws (t : TParser α) := spaces *> t <* spaces
+
+def reserved := 
+  #["infixl", "infixr","let", "rec", "in", "fn", "fun", "=", "if", "else", "then", "->", ";;"]
+
 open ASCII in def ID' : TParser String :=
   withErrorMessage "identifier" do
       (· ++ ·)
-  <$> (Char.toString <$> alpha)
+  <$> (Char.toString <$> alpha')
   <*> foldl String.push "" alphanum'
 
 def ID : TParser String := do
   let id <- ID'
   if reserved.contains id then throwUnexpectedWithMessage none s!"expected identifier, not keyword {id}"
-  else return id
+  else ws $ pure id
+abbrev kw (s : String) : TParser Unit := ws 
+                                         $ withBacktracking
+                                         $ withErrorMessage "keyword"
+                                         $ string s
+                                         *> notFollowedBy alphanum'
 
-def spaces : TParser Unit :=
-  dropMany <| tokenFilter [' ', '\n', '\r', '\t'].contains
-abbrev ws (t : TParser α) := spaces *> t <* spaces
+abbrev LET   := kw "let"
+abbrev IN    := kw "in"
+abbrev FUN   := kw "fun"
+abbrev EQ    := kw "="
+abbrev IF    := kw "if"
+abbrev ELSE  := kw "else"
+abbrev THEN  := kw "then"
+abbrev ARROW := kw "->"
+abbrev COMMA := kw ","
+abbrev REC   := kw "rec"
+abbrev END   := kw ";;"
 
-abbrev kw (s : String) : TParser String := withErrorMessage "keyword" do spaces *> string s <* spaces
-abbrev LET   := drop 1 $ kw "let"
-abbrev IN    := drop 1 $ kw "in"
-abbrev FUN   := drop 1 $ kw "fun"
-abbrev EQ    := drop 1 $ kw "="
-abbrev IF    := drop 1 $ kw "if"
-abbrev ELSE  := drop 1 $ kw "else"
-abbrev THEN  := drop 1 $ kw "then"
-abbrev ARROW := drop 1 $ kw "->"
-abbrev COMMA := spaces *> kw ","
+abbrev ADD   := "+"
+abbrev SUB   := "-"
+abbrev MUL   := "*"
+abbrev DIV   := "/"
+abbrev DOL   := "$"
+abbrev ATT   := "@@"
+
+abbrev INFIXL := kw "infixl"
+abbrev INFIXR := kw "infixr"
+
 end Lexing
 
-abbrev Symbol := String
-inductive Expr where
-  | CI (i : Int)       | CS (s : String)        | CB (b : Bool) | CUnit
-  | App (e₁ e₂ : Expr) | Cond (e₁ e₂ e₃ : Expr) | Let (a : Symbol) (e₁ e₂ : Expr)
-  | Var (s : Symbol)   | Fun (a : Symbol) (e : Expr)
-  | Prod' (e₁ e₂ : Expr)
-deriving Repr, BEq, Nonempty
-
-instance : Inhabited Expr := ⟨Expr.CUnit⟩
-
-def List.reduce [Inhabited α] (f : α -> α -> α) (xs : List α) :=
+def List.mapReduce! [Inhabited β] (mapf : α -> β) (f : β -> β -> β) (xs : List α) : β :=
   match xs with
-  | [] => default | [x] => x
-  | x :: x' :: xs => reduce f (f x x' :: xs)
+  | [] => default
+  | x :: xs => xs.foldl (flip $ flip f ∘ mapf) (mapf x)
 
 namespace Parsing
 open Lexing Expr
-
+section helper
+variable {ε σ τ m α} 
+         [Parser.Stream σ τ] 
+         [Parser.Error ε σ τ] 
+         [Monad m]
 /--
   `chainl1 p op` parses *one* or more occurrences of `p`, separated by `op`. Returns
   a value obtained by a **left** associative application of all functions returned by `op` to the
   values returned by `p`.
+  - if there is exactly one occurrence of `p`, `p` itself is returned touched.
 -/
-partial def chainl1  [Parser.Stream σ τ] [Parser.Error ε σ τ] [Monad m]
+partial def chainl1 
   (p : ParserT ε σ τ m α)
   (op : ParserT ε σ τ m (α -> α -> α)) : ParserT ε σ τ m α := do
   let x <- p; rest x where
   rest x :=
     (do let f <- op; let y <- p; rest (f x y)) <|> pure x
-def chainl [Parser.Stream σ τ] [Parser.Error ε σ τ] [Monad m]
+
+partial def chainr1
   (p : ParserT ε σ τ m α)
-  (op : ParserT ε σ τ m (α -> α -> α))
-  (x : α) : ParserT ε σ τ m α := chainl1 p op <|> return x
+  (op : ParserT ε σ τ m (α -> α -> α)) : ParserT ε σ τ m α := do
+  let x <- p; rest x where
+  rest x :=
+    (do let f <- op; chainr1 p op <&> f x) <|> pure x
+
+@[inline] def η₂ s :=
+  fun e₁ e₂ => App (App s e₁) e₂
+
+@[inline] def infixOp (op : Symbol) (e : α -> α -> α) : TParser $ α -> α -> α :=
+  (kw op) *> pure e
+
+@[inline] def link s := η₂ $ Var s
+
+@[inline] def buildOpParser
+  (p : TParser α)
+  (table : OpTable α)
+  : TParser α := table.foldl (init := p) fun a (_, s) (e, assoc) =>
+    match assoc with
+    | .leftAssoc => chainl1 a $ infixOp s e
+    | .rightAssoc => chainr1 a $ infixOp s e
+
+def first'
+  (ps : Array $ ParserT ε σ τ m α)
+  (combine : ε → ε → ε := fun _ => id)
+  : ParserT ε σ τ m α := do
+  let rec go n (h : n <= ps.size) e s :=
+    match _ : n with
+    | 0 => return .error s e
+    | m + 1 => 
+      let pss := ps.size
+      have : m < pss := Nat.le_trans (Nat.lt.base _) h
+      let savePos := Stream.getPosition s
+      ps[pss - m.succ] s >>= fun
+      | .ok s v => return .ok s v
+      | .error s f =>
+        go m (Nat.le_of_lt this) (combine e f) (Stream.setPosition s savePos)
+  go ps.size (Nat.le.refl) (Error.unexpected (<- getPosition) none)
+
+end helper
+
+open Associativity in
+def opTable : OpTable Expr := .ofArray (cmp := opIndexOrd.compare)
+  #[ ((0   , DOL)     , (App       , rightAssoc))
+   , ((0   , ATT)     , (App       , rightAssoc))
+   , ((50  , "=")     , (link "eq" , leftAssoc))
+   , ((65  , ADD)     , (link "add", leftAssoc))
+   , ((65  , SUB)     , (link "sub", leftAssoc))
+   , ((70  , MUL)     , (link "mul", leftAssoc))
+   , ((70  , DIV)     , (link "div", leftAssoc))]
+
 mutual
-private partial def atom : TParser Expr :=
-  first [ parenthesized (spaces *> pure CUnit)
-        , parenthesized prodExp
-        , ws varExp
-        , ws letExp
-        , ws funExp
-        , ws condExp
-        , ws intExp
-        , ws strExp]
 
-
-private partial def exp : TParser Expr :=
+private partial def funapp : TParser Expr := 
   chainl1 atom (pure App)
 
+private partial def atom : TParser Expr :=
+  first' $ #[ parenthesized prodExp
+            , letrecExp                  , letExp
+            , fixpointExp                , funExp
+            , condExp                    , intExp
+            , strExp                     , varExp
+            , parenthesized opSection]
+            |>.map ws
+
 private partial def prodExp : TParser Expr := do
-  let e <- exp
-  let es <- takeMany (COMMA *> exp)
-  match es.toList with
-  | [] => pure e | e' :: es => pure $ es.foldl Prod' (Prod' e e')
+  let es <- sepBy COMMA parseExpr
+  return match h : es.size with
+         | 0 => CUnit
+         | 1 => es[0]
+         | _ + 2 => es[0:es.size - 1].foldr Prod' es[es.size - 1]
 
-private partial def between (l : Char) (t : TParser Expr) (r : Char) : TParser Expr :=
- spaces *> char l *> spaces *> t <* spaces <* char r <* spaces
-private partial def parenthesized (t : TParser Expr) : TParser Expr := between '(' t ')'
+private partial
+def between (l : Char) (t : TParser Expr) (r : Char) : TParser Expr :=
+  ws (char l) *> t <* ws (char r)
+private partial
+def parenthesized (t : TParser Expr) : TParser Expr := between '(' t ')'
 
-private partial def intExp  : TParser Expr := INT             >>= pure ∘ CI
-private partial def strExp  : TParser Expr := do
-  let s <- char '"'
-        *> foldl String.push "" (tokenFilter (not ∘ ['"'].contains))
-        <* char '"'                                           return CS s
-private partial def varExp  : TParser Expr :=
+private partial def intExp      : TParser Expr := ws INT >>= pure ∘ CI
+
+private partial def strExp      : TParser Expr :=
+  CS <$> (char '"' *>
+            foldl .push "" (tokenFilter (· != '"'))
+          <* char '"')
+
+private partial def varExp      : TParser Expr :=
   ID >>= pure ∘ fun
-         | "true"                                             => CB true
-         | "false"                                            => CB false
-         | v                                                  => Var v
-private partial def letExp  : TParser Expr := do
-  LET; let id <- ID; EQ; let e₁ <- exp; IN; let e₂ <- exp     return Let id e₁ e₂
-private partial def funExp  : TParser Expr := do
-  FUN; let var <- ID; ARROW; let e <- exp                     return Fun var e
-private partial def condExp : TParser Expr := do
-  IF; let c <- exp; THEN; let e₁ <- exp; ELSE; let e₂ <- exp  return Cond c e₁ e₂
+          | "true"                => CB true
+          | "false"               => CB false
+          | v                     => Var v
+
+private partial def opMatcher (arr : Array $ Nat × String) : TParser OpIndex :=
+  first' $ arr.map fun (prec, s) => string s >>= pure ∘ (prec, ·)
+
+private partial def opSection   : TParser Expr := do
+  let e₁ <- option? parseExpr
+  let tb <- get
+  let k <- opMatcher tb.keysArray
+  let e₂ <- option? parseExpr
+  if let some (op, _) := tb.get? k then
+    match e₁, e₂ with
+    | some e₁, some e₂ =>         return op e₁ e₂
+    | _, some e₂ =>               return Fun "y" $ (flip op $ e₂) $ Var "y"
+    | some e₁, _ =>               return Fun "x" $ op e₁ $ Var "x"
+    | none, none =>               return Fun "x" $ Fun "y" $ op (Var "x") (Var "y")
+  else unreachable!
+
+private partial def letExp      : TParser Expr := do
+  LET let id <- ID
+      let a <- takeMany ID
+  EQ; let e₁ <- parseExpr
+  IN; let e₂ <- parseExpr         return Let id (a.foldr Fun e₁) e₂
+
+private partial def letrecExp   : TParser Expr := do
+  LET; REC
+      let id <- ID
+      let a <- takeMany ID
+  EQ  let e₁ <- parseExpr
+  IN  let e₂ <- parseExpr         return Let id (Fix $ Fun id $ a.foldr Fun e₁) e₂
+
+private partial def fixpointExp : TParser Expr := do
+  REC;
+  match <-option? parseExpr with
+  | some e =>                     return Fixcomb e
+  | none   =>                     return Var "rec"
+
+private partial def funExp      : TParser Expr := do
+  FUN   let var <- takeMany1 ID
+  ARROW let e <- parseExpr        return var.foldr Fun e
+
+private partial def condExp     : TParser Expr := do
+  IF   let c <- parseExpr
+  THEN let e₁ <- parseExpr
+  ELSE let e₂ <- parseExpr        return Cond c e₁ e₂
+
+private partial def parseExpr : TParser Expr := 
+  buildOpParser funapp =<< get
 
 end
+
+def infixlDecl : TParser (Symbol × Expr) := do
+  INFIXL; let i <- intExp let s <- strExp
+  match s, i with
+  | CS op, CI i =>
+    let op := op.trim
+    ARROW let e <- parseExpr
+    modify (·.insert (i.toNat, op) (η₂ e, .leftAssoc))
+    return (op, e)
+  | _, _ => unreachable!
+
+def infixrDecl : TParser (Symbol × Expr) := do
+  INFIXR; let i <- intExp let s <- strExp
+  match s, i with
+  | CS op, CI i =>
+    let op := op.trim
+    ARROW let e <- parseExpr
+    modify (·.insert (i.toNat, op) (η₂ e, .rightAssoc))
+    return (op, e)
+  | _, _ => unreachable!
+
+def letDecl : TParser Binding := do
+  LET; let id <- ID; let a <- takeMany ID; EQ; let b <- parseExpr;  return (id, a.foldr Fun b)
+def letrecDecl : TParser Binding := do
+  LET;
+  REC; let id <- ID; let a <- takeMany ID; EQ; let b <- parseExpr;  return (id, Fix $ Fun id $ a.foldr Fun b)
+
+def value p := show TParser Binding from ("_", ·) <$> p
+
+def declaration := first' #[ letrecDecl
+                          , letDecl
+                          , infixlDecl
+                          , infixrDecl
+                          , value parseExpr]
+
+def module : TParser $ Array Binding :=
+  sepBy (optional END) declaration <* optional END
+
 def parse (s : String) : Except String Expr :=
-  match Parser.run (spaces *> exp <* endOfInput) s with
+  match spaces *> parseExpr <* endOfInput |>.run s |>.run' opTable with
   | .ok _ t    => pure t
   | .error _ e => throw (toString e)
 
-end Parsing
+def parseModule (s : String) : EStateM String (OpTable Expr) (Array Binding) := do
+  match spaces *> module <* endOfInput |>.run s |>.run (<- get) with
+  | (.ok _ t, s)    => set s *> pure t
+  | (.error _ e, _) => throw (toString e)
 
+end Parsing
 
 def List.rmDup [BEq α] [Hashable α] (l : List α) : List α :=
   let s : Std.HashSet α := ∅
@@ -133,7 +330,6 @@ def List.rmDup [BEq α] [Hashable α] (l : List α) : List α :=
     | [] => []
     | x :: xs => if x ∈ s then go s xs else x :: go (insert x s) xs
   go s l
-
 
 inductive TV where
   | mkTV : String -> TV deriving Repr, BEq, Ord, Hashable
@@ -150,11 +346,12 @@ infixr: 50 " ->' " => MLType.TArr
 infixr: 65 " ×'' " => MLType.TProd
 def MLType.toStr : MLType -> String
   | TVar a => toString a | TCon a => a
-  | a ×'' b => paren (arr? a) (toStr a) ++ " × " ++ paren (arr? b) (toStr b)
+  | a ×'' b => paren (prod? a) (toStr a) ++ " × " ++ toStr b
   | a ->' b =>
     paren (arr? a) (toStr a) ++ " → " ++ toStr b where
     paren b s := bif b then s!"({s})" else s
     arr? | TArr _ _ => true | _ => false
+    prod? | TProd _ _ => true | _ => false
 
 instance : ToString MLType := ⟨MLType.toStr⟩
 
@@ -164,23 +361,31 @@ inductive Scheme where
 instance : ToString Scheme where
   toString
   | .Forall [] t => toString t
-  | .Forall ts t => "∀ { " ++ (ts.foldl (init := "") fun a s => s!"{a}{s} ") ++ s!"}. {toString t}"
+  | .Forall ts t => s!"∀ {ts.mapReduce! toString (· ++ " " ++ ·)}. {toString t}"
+
+instance : Inhabited Scheme where
+  default := .Forall [] (MLType.TCon "False")
 
 namespace MLType open TV Expr
+
 inductive TypingError
   | NoUnify (t₁ t₂ : MLType)
   | Undefined (s : String)
-  | NonApplicable
   | WrongCardinal (n : Nat)
   | Duplicates (t : TV) (T : MLType) deriving Repr
 
 instance : ToString TypingError where
   toString
   | .NoUnify t₁ t₂ => s!"Can't unify type\n  {t₁}\nwith\n  {t₂}."
-  | .Undefined s   => s!"Variable\n  {s}\nis not in scope."
-  | .NonApplicable => s!"This expression is not applicable."
+  | .Undefined s   => s!"Variable\n  {s}\nis not in scope.\n\
+                         Note: use letrec or fixcomb if this is a recursive definition"
   | .WrongCardinal n => s!"Incorrect cardinality. Expected {n}"
-  | .Duplicates (mkTV a) b =>  s!"Unbounded fixpoint constructor does not exist in a strongly normalized system.\nNote: unifying {a} and {b} results in μ{a}. {b}, which isn't allowed."
+  | .Duplicates (mkTV a) b =>
+    s!"\
+    Unbounded fixpoint constructor does not exist in a strongly normalized system.\n\
+    Note: unifying {a} and {b} results in μ{a}. {b}, which isn't allowed.\n\
+    Note: recursion is supported primitively via letrec \n\
+    Note: or unsafely via fixpoint combinator `rec`"
 open TypingError
 abbrev Env := Std.HashMap String Scheme
 abbrev Infer σ := StateRefT Nat $ EST TypingError σ
@@ -195,28 +400,31 @@ def curry : MLType -> MLType
 where
   go | t₃ ×'' t₄ => go t₃ ++ go t₄ | t => [t]
 
+local instance : CoeHead String TV := ⟨mkTV⟩
+local instance : CoeTail TV MLType := ⟨TVar⟩
+
 @[inline] abbrev tInt := TCon "Int"
 @[inline] abbrev tBool := TCon "Bool"
 @[inline] abbrev tString := TCon "String"
 @[inline] abbrev tUnit := TCon "Unit"
-@[inline] abbrev typeOf (e : Env) s := e.get? s
+
 abbrev dE : List (String × Scheme) :=
-  [ ("add'", .Forall []      $ tInt ×'' tInt ->' tInt)
-  , ("sub'", .Forall []      $ tInt ×'' tInt ->' tInt)
-  , ("mul'", .Forall []      $ tInt ×'' tInt ->' tInt)
-  , ("div'", .Forall []      $ tInt ×'' tInt ->' tInt)
-  , ("eq'",  .Forall [⟨"α"⟩] $ TVar ⟨"α"⟩ ×'' TVar ⟨"α"⟩ ->' tBool)
-  , ("not",  .Forall []      $ tBool ->' tBool)
-  , ("id",   .Forall [⟨"α"⟩] $ TVar ⟨"α"⟩ ->' TVar ⟨"α"⟩)
-  , ("zero", .Forall []      $ tInt)
-  , ("succ", .Forall []      $ tInt ->' tInt)]
+  [ ("rec"  , .Forall ["α"] $ ("α" ->' "α") ->' "α")
+  , ("__add", .Forall []    $ tInt ×'' tInt ->' tInt)
+  , ("__sub", .Forall []    $ tInt ×'' tInt ->' tInt)
+  , ("__mul", .Forall []    $ tInt ×'' tInt ->' tInt)
+  , ("__div", .Forall []    $ tInt ×'' tInt ->' tInt)
+  , ("__eq" , .Forall ["α"] $ "α" ×'' "α" ->' tBool)
+  , ("not"  , .Forall []    $ tBool ->' tBool)
+  , ("id"   , .Forall ["α"] $ "α" ->' "α")
+  , ("succ" , .Forall []    $ tInt ->' tInt)]
 
-
+variable {σ : Type}
 
 abbrev defaultE : Env := .ofList $
   dE.foldl (init := []) fun a p@(sym, .Forall c ty) =>
-    if sym.endsWith "\'"
-    then p :: (sym.dropRight 1, .Forall c $ curry ty) :: a
+    if sym.startsWith "__"
+    then p :: (sym.drop 2, .Forall c $ curry ty) :: a
     else p :: a
 
 class Rewritable (α : Type) where
@@ -225,6 +433,7 @@ class Rewritable (α : Type) where
 open Rewritable
 
 namespace Rewritables
+
 def diff [BEq α] [Hashable α] (s₁ s₂ : Std.HashSet α) :=
   s₂.fold (fun a s => if s ∈ s₁ then s₁.erase s else a) s₁
 instance [BEq α] [Hashable α] : SDiff (Std.HashSet α) := ⟨diff⟩
@@ -306,6 +515,14 @@ def lookupEnv (s : String) (E : Env) : Infer σ (Subst × MLType) :=
 infix :50 " ∈ₑ " => lookupEnv
 
 mutual
+/--
+  perform exactly 1 step of sequential inferrence in CPS style.
+  Sequential inferrence is manually unwinded in
+  `infer` e.g. `If` `Fix` branch.
+  It is done this way so that Lean doesn't complain about termination problem.
+    (it can get complicated as `infer1` is mutually recursive with `infer`)
+  - returns a continuation and a modified substitution map.
+-/
 def infer1 (E : Env) : (Subst × (MLType -> MLType)) -> Expr -> Infer σ (Subst × (MLType -> MLType))
   | (s, contT), e => do
     let (s', t) <- infer (apply s E) e
@@ -318,6 +535,24 @@ def infer (E : Env) : Expr -> Infer σ (Subst × MLType)
     let E'       := E.insert x (.Forall [] tv)
     let (s₁, t₁) <- infer E' e
     pure (s₁, apply s₁ tv ->' t₁)
+
+  | Fixcomb e => do
+    let tv <- fresh
+    let tv' <- fresh
+    let (s₁, cont) <- infer1 E (∅, id) e
+    let s₂ <- unify (apply s₁ (cont tv')) ((tv ->' tv) ->' tv)
+    pure (s₂ ∪' s₁, apply s₂ tv')
+
+  | Fix (Fun fname fbody) => do
+    let tv <- fresh
+    let E' := E.insert fname (.Forall [] tv)
+    let (s₁, t₁) <- infer E' fbody
+    let s₂ <- unify (apply s₁ tv) t₁
+    let s := s₂ ∪' s₁
+    pure (s₂ ∪' s₁, apply s tv)
+  | Fix e => do
+    let (s₁, t₁) <- infer E e
+    pure (s₁, t₁)
 
   | App e₁ e₂ => do
     let tv       <- fresh
@@ -360,12 +595,15 @@ def runInfer1 (e : Expr) (E : Env) : Except TypingError Scheme :=
   | .error e => throw e
   | .ok  res => pure $ closed res
 
-def check1 (s : String) (E : Env := ∅) : String :=
+def inferToplevel (b : Array Binding) (E : Env) : Except TypingError Env :=
+  b.foldlM (init := E) fun E (id, expr) => runInfer1 expr E <&> E.insert id
+
+def check1 (s : String) (E : Env := defaultE) : String :=
   match Parsing.parse s with
   | .error e => toString e
   | .ok e    =>
     match runInfer1 e E with
-    | .error e => toString e
+    | .error e' => toString e' ++ s!"AST: {reprStr e}"
     | .ok    s => toString s
 
 def asType : MLType -> Type
@@ -380,66 +618,84 @@ structure VEnv where
 
 inductive Value where
   | VI (i : Int) | VB (b : Bool) | VS (s : String) | VU
-  | VF (s : Symbol) (e : Expr) (e : VEnv)
+  | VF (s : Symbol) (E : Expr) (e : VEnv)
+  | VFRec (s: Symbol) (e : Expr) (E : VEnv)
   | VOpaque (s : Nat)
   | VEvalError (s : String)
-  | VP (e₁ e₂ : Value) deriving Nonempty, Repr
+  | VP (e₁ e₂ : Value) deriving Nonempty
 end
-instance : Inhabited Value := ⟨.VEvalError "something wrong during evaluation. Likely implementation error."⟩
-def Value.toStr
-  | VI v | VB v | VS v => reprStr v | VU => toString ()
+instance : Inhabited Value := ⟨.VEvalError "something wrong during evaluation.\n\
+                                            Note: Likely implementation error or a breach of type safety\n\
+                                            Note: The type system is unsound by design\n\
+                                            Note: because the primitive `rec` fixpoint combinator is present\n"⟩
+def Value.toStr : Value -> String
+  | VI v | VB v => toString v | VU => toString ()
+  | VS v => reprStr v
   | VEvalError s => s
-  | VOpaque s  => s!"<${s}::opaque>"
-  | VF _ _ _   => "<fun>"
-  | VP v₁ v₂   => toStr v₁ ++ "," ++ toStr v₂
+  | VOpaque s   => s!"<${s}::prim>"
+  | VF _ _ _    => "<fun>"
+  | VFRec _ _ _ => "<recfun>"
+  | VP v₁ v₂    => paren (prod? v₁) (toStr v₁) ++ "," ++ toStr v₂ where
+    paren b s := bif b then s!"({s})" else s
+    prod? | VP _ _ => true | _ => false
 
-@[inline, always_inline]abbrev Value.flatten1 : Value -> List Value
-  | VP v₁ v₂ => [v₁] ++ [v₂]
-  | t@_ => [t]
-
-def binop : Nat -> Int -> Int -> Int
-  | 0 => (· + ·) | 1 => (· - ·) | 2 => (· * ·) | 3 => (· / ·)
-  | _ => panic! "Not defined"
+def binop (n : Nat) (h : n ∈ [1,2,3,4]) : Int -> Int -> Int :=
+  match n with
+  | 1 => (· + ·) | 2 => (· - ·) | 3 => (· * ·) | 4 => (· / ·)
 
 open Value in instance : ToString Value := ⟨Value.toStr⟩ in
-def callForeign (as : List Value) : Nat -> Value
-  | t@0 | t@1 | t@2 | t@3 =>
-    if let (VI i, VI i') := (as[0]!, as[1]!) then
-      VI $ (binop t) i i'
+def callForeign (as' : Value) (n : Nat) : Value :=
+  let as := match as' with | VP v₁ v₂ => [v₁, v₂] | _ => [as']
+  have : List.length as > 0 := by cases as' <;> simp[as]
+  match h : n with
+  | 1 | 2 | 3 | 4 =>
+    if let t@(VI i, VI i') := (as[0], as[1]!) then
+      VI $ (binop n $ by simp[h]) i i'
     else unreachable!
-
-  | 4 =>
-    if let (VB b) := as[0]! then
+  | 5 =>
+    if let (VB b) := as[0] then
       VB $ b.not
     else unreachable!
-
-  | 5 =>
+  | 6 =>
     let rec go : Value -> Value -> Except Value Bool
       | VI i, VI i' | VB i, VB i' | VS i, VS i' | VOpaque i, VOpaque i' =>
         pure $ i == i'
       | VU, VU => pure true
       | VF .., VF .. => throw $ VEvalError s!"equality handler is not implemented for function type"
       | VP l r, VP l' r' => (· && ·) <$> go l l' <*> go r r'
-      | _, _ => unreachable!
-    match go as[0]! as[1]! with
+      | x, y => unreachable!
+    match go as[0] as[1]! with
     | .ok x => VB x | .error e => e
+  | 7 => if let (VI i) := as[0] then VI $ i + 1 else unreachable!
+
   | n => .VOpaque n
 in
 partial def eval (E : VEnv) : Expr -> Except TypingError Value
   | CI v => pure $ VI v | CS v => pure $ VS v | CB v => pure $ VB v | CUnit => pure VU
   | Var x => match E.env.get? x with | some x => pure x | none => throw $ Undefined x
   | Fun x body => pure $ VF x body E
+  | Fix e | Fixcomb e =>
+    eval E e >>= fun
+    | VF fname fbody E' =>
+      pure $ VFRec fname fbody E'
+    | _ => unreachable!
   | App f a => do
-    let e' <- eval E f
-    match e' with
+    match <- eval E f with
     | VF s body E' =>
       let e <- eval E a
       let E' := E'.env.insert s e
       eval ⟨E'⟩ body
     | VOpaque n =>
       let a <- eval E a
-      pure $ callForeign a.flatten1 n
-    | _ => throw $ NonApplicable
+      pure $ callForeign a n
+    | self@(VFRec fname fbody E') =>
+      let e <- eval E a
+      let recE := E'.env.insert fname self
+      match fbody with
+      | Fun x body =>
+        eval ⟨recE.insert x e⟩ body
+      | _ => unreachable!
+    | _ => unreachable!
   | Let x e body => do
     let e' <- eval E e
     let E' := E.env.insert x e'
@@ -474,16 +730,18 @@ abbrev ag (prim : Symbol) (arity : {n // n > 1}) (primE : VEnv := ⟨∅⟩) : V
   arityGen prim arity primE
 
 def prim :=
-  [ ("id" ,   eval! "fun x -> x")
-  , ("add'",  .VOpaque 0)
-  , ("sub'",  .VOpaque 1)
-  , ("mul'",  .VOpaque 2)
-  , ("div'",  .VOpaque 3)
-  , ("not",   .VOpaque 4)
-  , ("eq'" ,  .VOpaque 5)]
+  [ ("id"   , eval! "fun x -> x")
+  , ("rec"  , .VOpaque 0)
+  , ("__add", .VOpaque 1)
+  , ("__sub", .VOpaque 2)
+  , ("__mul", .VOpaque 3)
+  , ("__div", .VOpaque 4)
+  , ("not"  , .VOpaque 5)
+  , ("__eq" , .VOpaque 6)
+  , ("succ" , .VOpaque 7)]
 def prim' : VEnv := ⟨.ofList prim⟩
 
-scoped macro n:term "of!" s:term : term => `(($n, (ag (String.push $n '\'') ⟨$s, by omega⟩ prim')))
+scoped macro n:term "of!" s:term : term => `(($n, (ag (String.append "__" $n) ⟨$s, by omega⟩ prim')))
 abbrev defaultVE : VEnv where
   env := .ofList $ prim
   ++ [ "add" of! 2
@@ -491,27 +749,107 @@ abbrev defaultVE : VEnv where
      , "mul" of! 2
      , "div" of! 2
      , "eq"  of! 2]
-  ++ [ ("zero",  eval! "0" prim')
-     , ("succ",  eval! "fun x -> add' (x,1)" prim')]
 
-def check1E (s : String) (E : Env := ∅) (VE : VEnv := ⟨∅⟩) : Except String String := do
-  let e <- Parsing.parse s
-  match runInfer1 e E, eval VE e with
-  | .error s, _ => throw $ toString s
-  | _, .error s => throw $ toString s
-  | .ok s, .ok r =>
-    pure $ toString r ++ " ⊢ " ++ toString s
+def evalToplevel (bs : Array Binding) (VE : VEnv) : Except TypingError VEnv :=
+  bs.foldlM (init := VE) fun VE@⟨env⟩ (id, e) => (VEnv.mk ∘ env.insert id) <$> eval VE e
 
+def interpret (PE : OpTable Expr) (E : Env) (VE : VEnv) (s : String) : IO (OpTable Expr × Env × VEnv) := do
+  match Parsing.parseModule s PE with
+  | .ok bs PE => 
+     let E <- IO.ofExcept $ inferToplevel bs E |>.mapError toString
+     let VE@{env} <- IO.ofExcept $ evalToplevel bs VE |>.mapError toString
+     (PE, E, VE) <$ bs.forM fun (id, _) =>
+       match E.get? id, env.get? id with
+       | some t, some r => println! "{id} : {r} ⊢ {t}"
+       | _, _ => pure ()
+  | .error e _ => IO.throwServerError e
+
+section PP open PrettyPrint Alignment
+
+def EnvHeader := ["id", "type", "value"]
+def alignE : Align EnvHeader := (left, left, right)
+def genTable (E : Env) : VEnv -> TableOf EnvHeader
+  | {env := VE} => E.keysArray.map fun k =>
+    (k, toString $ E.get! k, toString $ VE.get! k)
+
+def PEnvHeader := ["op", "prec", "assoc"]
+def genTableOp (PE : OpTable Expr) : TableOf PEnvHeader :=
+  PE.toArray.map fun ⟨(prec, sym), (_, assoc)⟩ =>
+    (sym, toString prec, toString assoc)
+def alignPE : Align PEnvHeader := (left, right, left)
+
+def HelpHeader := ["cmd", "info"]
+def alignH : Align HelpHeader := (right,left)
+def helpMsg : TableOf HelpHeader :=
+  #[ ("#dump", "dump the REPL environment in table form")
+   , ("#load <path>+", "load src from <path>+ (that doesn't contain spaces) into REPL")
+   , ("#help", "show this help string")
+   , ("#ast <exp|decl>", "display the parsetree of <exp> or <decl>")]
+
+end PP
 end MLType
 
-open MLType IO in def main : IO Unit := do
-  let prompt := "λ> "
+open PrettyPrint (tabulate) in
+open MLType IO in
+def main : IO Unit := do
   setStdoutBuf false
+
+  let motd := "A basic language using Hindley-Milner type system with a naive interpreted implementation.\n\
+               For language specifications see source: Playbook/hm.lean\n\
+               Type #help;; to check available commands.\n\
+               To exit press <C-d> (Unix) or <C-z> if on Windows."
+  let mut prompt := "λ> "
+  let mut buf := ""
+
   let stdin <- IO.getStdin
+  let E <- mkRef defaultE
+  let VE <- mkRef defaultVE
+  let PE <- mkRef Parsing.opTable
+  println! motd
+
   repeat do
+    let pe <- PE.get
+    let e <- E.get
+    let ve <- VE.get
+
     print prompt
-    let input <- IO.FS.Stream.getLine stdin
+    prompt := ".. "
+
+    let input <- FS.Stream.getLine stdin
+    buf := buf ++ input |>.trimLeft
+
     if input.isEmpty then return ()
-    else if input.startsWith "\n" then continue
-    else match check1E input defaultE defaultVE with
-         | .error s | .ok s => println! s
+    if !input.trimRight.endsWith ";;" then continue
+    if input.startsWith "\n" then continue
+
+    if buf.startsWith "#help" then
+      print $ tabulate "Commands" {align := alignH} helpMsg
+    else if buf.startsWith "#ast" then
+      match (Parsing.parseModule $ buf.drop 4).run pe with
+      | .ok b _  => println! reprStr b
+      | .error e _ => println! e
+    else if buf.startsWith "#dump" then
+      println $ tabulate "REPL Environment" {align := alignE}  $ genTable e ve
+      print $ tabulate "Operators" {align := alignPE} $ genTableOp pe
+    else if buf.startsWith "#load" then
+      (buf.splitOn " ").tail |>.forM fun path => do
+        if !path.isEmpty then
+          try
+            let fs <- FS.readFile $ path.takeWhile fun c => c != ';' && !c.isWhitespace
+            println fs
+            let (PE', E', VE') <- interpret pe e ve fs
+            PE.set PE' *> E.set E' *> VE.set VE'
+          catch e => 
+            println! e;
+            println! 
+              PrettyPrint.Text.bold 
+                "NOTE: Evaluation context is restore as there are errors.\n\
+                 Fix those then #load again to update it." true
+    else try
+      let (PE', E', VE') <- interpret pe e ve buf
+      PE.set PE' *> E.set E' *> VE.set VE'
+    catch e => println! e
+
+    buf := ""
+    prompt := "λ> "
+
